

**Problem 1.**

Let  $\phi(x) = a_d x^d + a_{d-1} x^{d-1} + \cdots + a_1 x + a_0$  and  $\psi(x) = b_e x^e + b_{e-1} x^{e-1} + \cdots + e_1 x + e_0$ . Without the loss of generality suppose  $d \geq e$ . Now:

$$\begin{aligned} H\left(\frac{\phi(\frac{m}{n})}{\psi(\frac{m}{n})}\right) &\leq H\left(\frac{n^d \phi(\frac{m}{n})}{n^d \psi(\frac{m}{n})}\right) \\ &= \max\{|a_d m^d + \cdots + a_1 m n^{d-1} + a_0 n^d|, |b_e m^e n^{d-e} + \cdots + e_1 m n^{d-1} + e_0 n^d|\} \end{aligned}$$

Knowing  $H(\frac{m}{n}) = \max\{|m|, |n|\}$ , then  $m^x n^{d-x} \leq H(\frac{m}{n})^d$ :

$$\begin{aligned} \max\{|a_d m^d + \cdots + a_1 m n^{d-1} + a_0 n^d|, |b_e m^e n^{d-e} + \cdots + e_1 m n^{d-1} + e_0 n^d|\} &\leq \\ \max\{|a_d + \cdots + a_1 + a_0|, |b_e + \cdots + b_1 + b_0|\} H\left(\frac{m}{n}\right)^d & \end{aligned}$$

Putting  $k = \max\{|a_d + \cdots + a_1 + a_0|, |b_e + \cdots + b_1 + b_0|\}$ , we get:

$$\begin{aligned} H\left(\frac{\phi(\frac{m}{n})}{\psi(\frac{m}{n})}\right) &\leq k H\left(\frac{m}{n}\right)^d \\ \implies h\left(\frac{\phi(\frac{m}{n})}{\psi(\frac{m}{n})}\right) &\leq d h\left(\frac{m}{n}\right) + \log(k) \end{aligned}$$

**Problem 2.**

**Problem 3.**

(i) We know that:

$$4h(P) - k \leq h(2P) \leq 4h(P) + k$$

Where  $k$  is not dependent on  $P$ . Thus:

$$|h(2P) - 4h(P)| \leq k \tag{1}$$

Now for every  $n$  we have that:

$$\left| \frac{1}{4^n} h(2^n P) - \frac{1}{4^{n-1}} h(2^{n-1} P) \right| = \frac{1}{4^n} |h(2^n P) - 4h(2^{n-1} P)|$$

Using (1) with  $P = 2^{n-1} P$ :

$$\frac{1}{4^n} |h(2^n P) - 4h(2^{n-1} P)| \leq \frac{1}{4^n} k$$

This means that for any  $\epsilon > 0$ , there exists some  $n$  such that  $\frac{k}{4^n} \leq \epsilon$ , meaning there exists some index  $n$  such that for any term with index  $i > n$  in the sequence  $\{a_n\} = \{\frac{1}{4^n} h(2^n P)\}_{n=1}^\infty$ , we have that  $|a_i - a_{i-1}| < \epsilon$ , meaning that this sequence is Cauchy, which shows that it has a limit in  $\mathbb{R}$ , hence  $\hat{h}(P)$  is well-defined.

(ii) Using  $h(2P) \geq 4h(P) - k$  we get:

$$\begin{aligned}
h(2^n P) &\geq 4h(2^{n-1}P) - k \geq 4^2 h(2^{n-2}P) - (4+1)k \\
&\geq 4^3 h(2^{n-3}P) - (4^2 + 4 + 1)k \\
&\vdots \\
&\geq 4^n h(P) - (4^{n-1} + 4^{n-2} + \dots + 4 + 1)k
\end{aligned}$$

On the other hand using  $h(2P) \leq 4h(P) + k$  we get:

$$\begin{aligned}
h(2^n P) &\leq 4h(2^{n-1}P) + k \leq 4^2 h(2^{n-2}P) + (4+1)k \\
&\leq 4^3 h(2^{n-3}P) + (4^2 + 4 + 1)k \\
&\vdots \\
&\leq 4^n h(P) + (4^{n-1} + 4^{n-2} + \dots + 4 + 1)k
\end{aligned}$$

Meaning:

$$\begin{aligned}
|\hat{h}(P) - h(P)| &= \left| \lim_{n \rightarrow \infty} \frac{1}{4^n} h(2^n P) - h(P) \right| \\
&\leq \left| \lim_{n \rightarrow \infty} h(P) + \frac{4^{n-1} + \dots + 4 + 1}{4^n} k - h(P) \right| \\
&= \left| \lim_{n \rightarrow \infty} \frac{4^{n-1} + \dots + 4 + 1}{4^n} k \right|
\end{aligned}$$

Now there exists a  $C > 0$  such that:

$$\left| \lim_{n \rightarrow \infty} \frac{4^{n-1} + \dots + 4 + 1}{4^n} k \right| < C$$

Then we have:

$$|\hat{h}(P) - h(P)| \leq C$$

(iii)

(iv) If  $P$  is of finite order, then the set of points  $2^n P$  is finite, meaning that the set  $\{h(2^n P) | n \in \mathbb{N}\}$  has finite elements. This means that with increase of  $n$ ,  $\frac{1}{4^n} h(2^n P)$  decreases and its limit is 0. Therefore  $\hat{h}(P) = 0$ . Conversely, if  $\hat{h}(P) = 0$ , then by part (iii), we have that  $\hat{h}(mP) = m^2 \hat{h}(P) = 0$  for any  $m \in \mathbb{Z}$ . Using part (ii) we get:

$$|\hat{h}(mP) - h(mP)| < C$$

for any  $P$  and any  $m$ . But we have:

$$|\hat{h}(mP) - h(mP)| = |-h(mP)| = h(mP) < C$$

For any  $m \in \mathbb{Z}$ . But we know that the set  $\{Q \in E | h(Q) < C\}$  is finite. This means that the set  $\{mP | m \in \mathbb{Z}\}$  is finite, which means that  $P$  is of finite order.